\documentclass{article}
\usepackage{amsmath}
\usepackage{mathtools}
\usepackage{amssymb}
\usepackage{newunicodechar}
\usepackage{newunicodechar}
\newunicodechar{ε}{\ensuremath{\varepsilon}}
\newunicodechar{•}{\ensuremath{\bullet}}
\usepackage{ifthen}
\usepackage{mathpartir}
\newboolean{explanation}
\setboolean{explanation}{false}
\newcommand\explainabove[2]{\overset{\overset{%
\clap{\text{\scriptsize #2}}}%
{\downarrow}}{#1}}
\newcommand\explainbelow[2]{\underset{\underset{%
\clap{\text{\scriptsize #2}}}%
{\uparrow}}{#1}}
\newcommand\negate[1]{%
  \ifthenelse{\boolean{#1}}{%
    \setboolean{#1}{false}%
    }{%
    \setboolean{#1}{true}%
    }%
}
\newcommand\explain[2]{%
  \ifthenelse{\boolean{explanation}}{%
    \explainabove{#1}{#2}%
  }{%
    \explainbelow{#1}{#2}%
  }
  \negate{explanation}
}
\begin{document}
\subsection{myProof}
\begin{mathpar}\mprset{flushleft}
[x] • ε\explain={⟨ Left neutrality ]}
([ε] • x) • ε\explain={⟨ Left neutrality ]}
((ε • ε) • x) • ε\explain={⟨ Associativity ]}
(ε • ε) • x • ε\explain={⟨ Associativity ]}
ε • [ε • x • ε]\explain={[ Associativity ⟩}
ε • [(ε • x) • ε]\explain={[ Right neutrality ⟩}
ε • [ε • x]\explain={[ Left neutrality ⟩}
ε • x
\end{mathpar}
\subsection{myProof2}
\begin{mathpar}\mprset{flushleft}
x • ([x] • ε)\explain={⟨ Left neutrality ]}
x • ([ε • x] • ε)\explain={⟨ Right neutrality ]}
[x] • ((ε • x) • ε) • ε\explain={⟨ Left neutrality ]}
[ε • x] • ((ε • x) • ε) • ε\explain={⟨ Right neutrality ]}
(ε • x) • ε • [((ε • x) • ε) • ε]\explain={⟨ Associativity ]}
(ε • x) • ε • (ε • x • [ε • ε])\explain={[ Left neutrality ⟩}
((ε • x) • ε) • (ε • x) • ε\explain={⟨ Associativity ]}
[ε • x] • ε • (ε • x) • ε\explain={[ Left neutrality ⟩}
x • (ε • [(ε • x) • ε])\explain={[ Right neutrality ⟩}
x • (ε • [ε • x])\explain={[ Left neutrality ⟩}
x • ε • x
\end{mathpar}
\subsection{myProof3}
\begin{mathpar}\mprset{flushleft}
x • (y • (z • [a]))\explain={⟨ Left neutrality ]}
x • (y • (z • [ε • a]))\explain={⟨ Right neutrality ]}
x • (y • ([z] • (ε • a) • ε))\explain={⟨ Left neutrality ]}
x • (y • ([ε • z] • (ε • a) • ε))\explain={⟨ Right neutrality ]}
x • ([y] • ((ε • z) • ε) • (ε • a) • ε)\explain={⟨ Left neutrality ]}
x • ([ε • y] • ((ε • z) • ε) • (ε • a) • ε)\explain={⟨ Right neutrality ]}
[x] • ((ε • y) • ε) • ((ε • z) • ε) • (ε • a) • ε\explain={⟨ Left neutrality ]}
[ε • x] • ((ε • y) • ε) • ((ε • z) • ε) • (ε • a) • ε\explain={⟨ Right neutrality ]}
(ε • x) • ε • ((ε • y) • ε • [((ε • z) • ε) • (ε • a) • ε])\explain={⟨ Associativity ]}
(ε • x) • ε • ((ε • y) • ε • (ε • z • (ε • [(ε • a) • ε])))\explain={⟨ Associativity ]}
(ε • x) • ε • ((ε • y) • ε • (ε • z • [ε • ε • a • ε]))\explain={[ Associativity ⟩}
(ε • x) • ε • ((ε • y) • ε • (ε • z • [(ε • ε) • a • ε]))\explain={[ Associativity ⟩}
(ε • x) • ε • ((ε • y) • ε • (ε • z • (([ε • ε] • a) • ε)))\explain={[ Left neutrality ⟩}
(ε • x) • ε • [((ε • y) • ε) • (ε • z) • (ε • a) • ε]\explain={⟨ Associativity ]}
(ε • x) • ε • (ε • y • (ε • [(ε • z) • (ε • a) • ε]))\explain={⟨ Associativity ]}
(ε • x) • ε • (ε • y • [ε • ε • z • (ε • a) • ε])\explain={[ Associativity ⟩}
(ε • x) • ε • (ε • y • [(ε • ε) • z • (ε • a) • ε])\explain={[ Associativity ⟩}
(ε • x) • ε • (ε • y • (([ε • ε] • z) • (ε • a) • ε))\explain={[ Left neutrality ⟩}
(ε • x • [ε]) • (ε • y) • (ε • z) • (ε • a) • ε\explain={⟨ Left neutrality ]}
[(ε • x) • ε • ε] • (ε • y) • (ε • z) • (ε • a) • ε\explain={[ Associativity ⟩}
((ε • x) • ε) • ε • (ε • y • (ε • z • (([ε] • a) • ε)))\explain={⟨ Left neutrality ]}
((ε • x) • ε) • ε • (ε • y • (ε • z • [((ε • ε) • a) • ε]))\explain={⟨ Associativity ]}
((ε • x) • ε) • ε • (ε • y • (ε • z • [(ε • ε) • a • ε]))\explain={⟨ Associativity ]}
((ε • x) • ε) • ε • (ε • y • (ε • z • (ε • [ε • a • ε])))\explain={[ Associativity ⟩}
((ε • x) • ε) • ε • (ε • y • [(ε • z) • ε • (ε • a) • ε])\explain={[ Associativity ⟩}
((ε • x) • ε) • ε • [(ε • y) • ((ε • z) • ε) • (ε • a) • ε]\explain={[ Associativity ⟩}
((ε • x) • ε) • ε • ((ε • y • (([ε] • z) • ε)) • (ε • a) • ε)\explain={⟨ Left neutrality ]}
((ε • x) • ε) • ε • ((ε • y • [((ε • ε) • z) • ε]) • (ε • a) • ε)\explain={⟨ Associativity ]}
((ε • x) • ε) • ε • ((ε • y • [(ε • ε) • z • ε]) • (ε • a) • ε)\explain={⟨ Associativity ]}
((ε • x) • ε) • ε • ((ε • y • (ε • [ε • z • ε])) • (ε • a) • ε)\explain={[ Associativity ⟩}
((ε • x) • ε) • ε • ([(ε • y) • ε • (ε • z) • ε] • (ε • a) • ε)\explain={[ Associativity ⟩}
([(ε • x) • ε] • ε) • (((ε • y) • ε) • (ε • z) • ε) • (ε • a) • ε\explain={[ Right neutrality ⟩}
([ε • x] • ε) • (((ε • y) • ε) • (ε • z) • ε) • (ε • a) • ε\explain={[ Left neutrality ⟩}
x • ε • (([(ε • y) • ε] • (ε • z) • ε) • (ε • a) • ε)\explain={[ Right neutrality ⟩}
x • ε • (([ε • y] • (ε • z) • ε) • (ε • a) • ε)\explain={[ Left neutrality ⟩}
x • ε • ((y • [(ε • z) • ε]) • (ε • a) • ε)\explain={[ Right neutrality ⟩}
x • ε • ((y • [ε • z]) • (ε • a) • ε)\explain={[ Left neutrality ⟩}
x • ε • (y • z • [(ε • a) • ε])\explain={[ Right neutrality ⟩}
x • ε • (y • z • [ε • a])\explain={[ Left neutrality ⟩}
(x • ε) • (y • z) • a
\end{mathpar}
\end{document}
