\documentclass{article}
\usepackage{amsmath}
\usepackage{newunicodechar}
\newunicodechar{ε}{\ensuremath{\varepsilon}}
\newunicodechar{•}{\ensuremath{\bullet}}
\begin{document}
\subsection{myProof}
\begin{align*}
[x] • ε
  & \quad \text{=⟨ Left neutrality ]}\\
([ε] • x) • ε
  & \quad \text{=⟨ Left neutrality ]}\\
((ε • ε) • x) • ε
  & \quad \text{=⟨ Associativity ]}\\
(ε • ε) • x • ε
  & \quad \text{=⟨ Associativity ]}\\
ε • [ε • x • ε]
  & \quad \text{=[ Associativity ⟩}\\
ε • [(ε • x) • ε]
  & \quad \text{=[ Right neutrality ⟩}\\
ε • [ε • x]
  & \quad \text{=[ Left neutrality ⟩}\\
ε • x
\end{align*}
\subsection{myProof2}
\begin{align*}
x • ([x] • ε)
  & \quad \text{=⟨ Left neutrality ]}\\
x • ([ε • x] • ε)
  & \quad \text{=⟨ Right neutrality ]}\\
[x] • ((ε • x) • ε) • ε
  & \quad \text{=⟨ Left neutrality ]}\\
[ε • x] • ((ε • x) • ε) • ε
  & \quad \text{=⟨ Right neutrality ]}\\
(ε • x) • ε • [((ε • x) • ε) • ε]
  & \quad \text{=⟨ Associativity ]}\\
(ε • x) • ε • (ε • x • [ε • ε])
  & \quad \text{=[ Left neutrality ⟩}\\
((ε • x) • ε) • (ε • x) • ε
  & \quad \text{=⟨ Associativity ]}\\
[ε • x] • ε • (ε • x) • ε
  & \quad \text{=[ Left neutrality ⟩}\\
x • (ε • [(ε • x) • ε])
  & \quad \text{=[ Right neutrality ⟩}\\
x • (ε • [ε • x])
  & \quad \text{=[ Left neutrality ⟩}\\
x • ε • x
\end{align*}
\subsection{myProof3}
\begin{align*}
x • (y • (z • [a]))
  & \quad \text{=⟨ Left neutrality ]}\\
x • (y • (z • [ε • a]))
  & \quad \text{=⟨ Right neutrality ]}\\
x • (y • ([z] • (ε • a) • ε))
  & \quad \text{=⟨ Left neutrality ]}\\
x • (y • ([ε • z] • (ε • a) • ε))
  & \quad \text{=⟨ Right neutrality ]}\\
x • ([y] • ((ε • z) • ε) • (ε • a) • ε)
  & \quad \text{=⟨ Left neutrality ]}\\
x • ([ε • y] • ((ε • z) • ε) • (ε • a) • ε)
  & \quad \text{=⟨ Right neutrality ]}\\
[x] • ((ε • y) • ε) • ((ε • z) • ε) • (ε • a) • ε
  & \quad \text{=⟨ Left neutrality ]}\\
[ε • x] • ((ε • y) • ε) • ((ε • z) • ε) • (ε • a) • ε
  & \quad \text{=⟨ Right neutrality ]}\\
(ε • x) • ε • ((ε • y) • ε • [((ε • z) • ε) • (ε • a) • ε])
  & \quad \text{=⟨ Associativity ]}\\
(ε • x) • ε • ((ε • y) • ε • (ε • z • (ε • [(ε • a) • ε])))
  & \quad \text{=⟨ Associativity ]}\\
(ε • x) • ε • ((ε • y) • ε • (ε • z • [ε • ε • a • ε]))
  & \quad \text{=[ Associativity ⟩}\\
(ε • x) • ε • ((ε • y) • ε • (ε • z • [(ε • ε) • a • ε]))
  & \quad \text{=[ Associativity ⟩}\\
(ε • x) • ε • ((ε • y) • ε • (ε • z • (([ε • ε] • a) • ε)))
  & \quad \text{=[ Left neutrality ⟩}\\
(ε • x) • ε • [((ε • y) • ε) • (ε • z) • (ε • a) • ε]
  & \quad \text{=⟨ Associativity ]}\\
(ε • x) • ε • (ε • y • (ε • [(ε • z) • (ε • a) • ε]))
  & \quad \text{=⟨ Associativity ]}\\
(ε • x) • ε • (ε • y • [ε • ε • z • (ε • a) • ε])
  & \quad \text{=[ Associativity ⟩}\\
(ε • x) • ε • (ε • y • [(ε • ε) • z • (ε • a) • ε])
  & \quad \text{=[ Associativity ⟩}\\
(ε • x) • ε • (ε • y • (([ε • ε] • z) • (ε • a) • ε))
  & \quad \text{=[ Left neutrality ⟩}\\
(ε • x • [ε]) • (ε • y) • (ε • z) • (ε • a) • ε
  & \quad \text{=⟨ Left neutrality ]}\\
[(ε • x) • ε • ε] • (ε • y) • (ε • z) • (ε • a) • ε
  & \quad \text{=[ Associativity ⟩}\\
((ε • x) • ε) • ε • (ε • y • (ε • z • (([ε] • a) • ε)))
  & \quad \text{=⟨ Left neutrality ]}\\
((ε • x) • ε) • ε • (ε • y • (ε • z • [((ε • ε) • a) • ε]))
  & \quad \text{=⟨ Associativity ]}\\
((ε • x) • ε) • ε • (ε • y • (ε • z • [(ε • ε) • a • ε]))
  & \quad \text{=⟨ Associativity ]}\\
((ε • x) • ε) • ε • (ε • y • (ε • z • (ε • [ε • a • ε])))
  & \quad \text{=[ Associativity ⟩}\\
((ε • x) • ε) • ε • (ε • y • [(ε • z) • ε • (ε • a) • ε])
  & \quad \text{=[ Associativity ⟩}\\
((ε • x) • ε) • ε • [(ε • y) • ((ε • z) • ε) • (ε • a) • ε]
  & \quad \text{=[ Associativity ⟩}\\
((ε • x) • ε) • ε • ((ε • y • (([ε] • z) • ε)) • (ε • a) • ε)
  & \quad \text{=⟨ Left neutrality ]}\\
((ε • x) • ε) • ε • ((ε • y • [((ε • ε) • z) • ε]) • (ε • a) • ε)
  & \quad \text{=⟨ Associativity ]}\\
((ε • x) • ε) • ε • ((ε • y • [(ε • ε) • z • ε]) • (ε • a) • ε)
  & \quad \text{=⟨ Associativity ]}\\
((ε • x) • ε) • ε • ((ε • y • (ε • [ε • z • ε])) • (ε • a) • ε)
  & \quad \text{=[ Associativity ⟩}\\
((ε • x) • ε) • ε • ([(ε • y) • ε • (ε • z) • ε] • (ε • a) • ε)
  & \quad \text{=[ Associativity ⟩}\\
([(ε • x) • ε] • ε) • (((ε • y) • ε) • (ε • z) • ε) • (ε • a) • ε
  & \quad \text{=[ Right neutrality ⟩}\\
([ε • x] • ε) • (((ε • y) • ε) • (ε • z) • ε) • (ε • a) • ε
  & \quad \text{=[ Left neutrality ⟩}\\
x • ε • (([(ε • y) • ε] • (ε • z) • ε) • (ε • a) • ε)
  & \quad \text{=[ Right neutrality ⟩}\\
x • ε • (([ε • y] • (ε • z) • ε) • (ε • a) • ε)
  & \quad \text{=[ Left neutrality ⟩}\\
x • ε • ((y • [(ε • z) • ε]) • (ε • a) • ε)
  & \quad \text{=[ Right neutrality ⟩}\\
x • ε • ((y • [ε • z]) • (ε • a) • ε)
  & \quad \text{=[ Left neutrality ⟩}\\
x • ε • (y • z • [(ε • a) • ε])
  & \quad \text{=[ Right neutrality ⟩}\\
x • ε • (y • z • [ε • a])
  & \quad \text{=[ Left neutrality ⟩}\\
(x • ε) • (y • z) • a
\end{align*}
\end{document}
